implement foundation for transpilation

example/misc.lua
@@ -1,0 +1,7 @@
+local ffi = require "ffi"
+ffi.cdef[[
+typedef struct {
+        int32_t internal_id
+        int32_t generation_counter
+} strong_id;
+]]
