example/output/location.lua
@@ -1,7 +1,18 @@
 local ffi = require("ffi")
 LOCATION = {}
 ---@param state data_arrays
+---@param id location_strong_id
+function LOCATION.is_valid(state, id)
+	local bounded = state.size_location > id.internal_id
+	if (not bounded) then return false end
+	local is_used = state.used_location_id[id.internal_id] == 1
+	local fresh = state.generation_counter_array_location[id.internal_id] == id.generation_counter
+	return bounded and is_used and fresh
+end
+---@param state data_arrays
 local function reserve_generation_array(state)
+	state.available_location_id = 0
+	state.used_location_id = ffi.new("uint8_t[?]", state.size_location)
 	state.generation_counter_array_location = ffi.new("int32_t[?]", state.size_location)
 end
 ---@class location_strong_id
@@ -30,4 +41,23 @@ end
 function LOCATION.reserve(state)
 	reserve_generation_array(state)
 	reserve_data_array_location_danger(state)
+end
+---@param state data_arrays
+---@returns location_strong_id
+function LOCATION.create(state)
+	local id = state.available_location_id
+	state.used_location_id[id] = 1
+	while state.used_location_id[state.available_location_id] ~= 0 do
+		assert(state.available_location_id < state.size_location)
+		state.available_location_id = state.available_location_id + 1
+	end
+	---@type location_strong_id
+	return ffi.new("struct strong_id", { id, state.generation_counter_array_location[id]  })
+end
+---@param state data_arrays
+---@param id location_strong_id
+function LOCATION.delete(state, id)
+	assert(LOCATION.is_valid(state, id))
+	state.used_location_id[id.internal_id] = 0
+	if (id.internal_id < state.available_location_id) then state.available_location_id = id.internal_id end
 end
