example/output/party_location.lua
@@ -1,7 +1,18 @@
 local ffi = require("ffi")
 PARTY_LOCATION = {}
 ---@param state data_arrays
+---@param id party_location_strong_id
+function PARTY_LOCATION.is_valid(state, id)
+	local bounded = state.size_party_location > id.internal_id
+	if (not bounded) then return false end
+	local is_used = state.used_party_location_id[id.internal_id] == 1
+	local fresh = state.generation_counter_array_party_location[id.internal_id] == id.generation_counter
+	return bounded and is_used and fresh
+end
+---@param state data_arrays
 local function reserve_generation_array(state)
+	state.available_party_location_id = 0
+	state.used_party_location_id = ffi.new("uint8_t[?]", state.size_party_location)
 	state.generation_counter_array_party_location = ffi.new("int32_t[?]", state.size_party_location)
 end
 ---@class party_location_strong_id
@@ -9,18 +20,49 @@ end
 ---@field generation_counter number
 
 ---@param state data_arrays
-local function reserve_link_array_party_location_party(state)
-	state.data_array_party_location_to_party = ffi.new("int32_t[?]", state.size_party_location)
-	state.data_array_party_location_from_party = ffi.new("int32_t[?]", state.size_party)
-end
----@param state data_arrays
 local function reserve_link_array_party_location_location(state)
 	state.data_array_party_location_to_location = ffi.new("int32_t[?]", state.size_party_location)
-	state.data_array_party_location_from_location = ffi.new("int32_t[?]", state.size_location)
+	state.data_array_party_location_one_from_location = ffi.new("int32_t[?]", state.size_location)
+end
+---@param state data_arrays
+local function reserve_link_array_party_location_party(state)
+	state.data_array_party_location_to_party = ffi.new("int32_t[?]", state.size_party_location)
+	state.data_array_party_location_many_from_party = {}
+	for i = 0, state.size_party - 1 do
+		state.data_array_party_location_many_from_party[i] = {}
+	end
 end
 ---@param state data_arrays
 function PARTY_LOCATION.reserve(state)
 	reserve_generation_array(state)
-	reserve_link_array_party_location_party(state)
 	reserve_link_array_party_location_location(state)
+	reserve_link_array_party_location_party(state)
+end
+---@param state data_arrays
+---@param location_link location_strong_id
+---@param party_link party_strong_id
+---@returns party_location_strong_id
+function PARTY_LOCATION.create(state, location_link, party_link)
+	local id = state.available_party_location_id
+	state.used_party_location_id[id] = 1
+	assert(LOCATION.is_valid(state, location_link))
+	assert(state.data_array_party_location_one_from_location[location_link.internal_id] == 0)
+	state.data_array_party_location_to_location[id] = location_link.internal_id
+	state.data_array_party_location_one_from_location[location_link.internal_id] = id
+	assert(PARTY.is_valid(state, party_link))
+	state.data_array_party_location_to_party[id] = party_link.internal_id
+	state.data_array_party_location_many_from_party[party_link.internal_id][id] = id
+	while state.used_party_location_id[state.available_party_location_id] ~= 0 do
+		assert(state.available_party_location_id < state.size_party_location)
+		state.available_party_location_id = state.available_party_location_id + 1
+	end
+	---@type party_location_strong_id
+	return ffi.new("struct strong_id", { id, state.generation_counter_array_party_location[id]  })
+end
+---@param state data_arrays
+---@param id party_location_strong_id
+function PARTY_LOCATION.delete(state, id)
+	assert(PARTY_LOCATION.is_valid(state, id))
+	state.used_party_location_id[id.internal_id] = 0
+	if (id.internal_id < state.available_party_location_id) then state.available_party_location_id = id.internal_id end
 end
