Main.lean
@@ -1,88 +1,63 @@
+import Std.Data.HashSet
+
 import LeanLuaDataArrays
 
-
--- format description
--- %object_name%
--- %field/link% %field_name% %field_type%
-
+def namespace_name (x : String) : String := x.toUpper
 def empty_table : String := "{}"
+def curly (s : String) := "{ " ++ s ++ " }"
 def tb : String := "\t"
 
-inductive value_t where
-  | uint8_t : value_t
-  | uint16_t : value_t
-  | uint32_t : value_t
-  | int8_t : value_t
-  | int16_t : value_t
-  | int32_t : value_t
-  | float : value_t
+inductive word_size where
+  | w1 : word_size
+  | w2 : word_size
+  | w4 : word_size
 
-def value_t.convert_to_string (x: value_t) : String :=
-  match x with
-  | uint8_t     => "uint8_t"
-  | uint16_t    => "uint16_t"
-  | uint32_t    => "uint32_t"
-  | int8_t      => "int8_t"
-  | int16_t     => "int16_t"
-  | int32_t     => "int32_t"
-  | float       => "float"
+inductive number_interpretation where
+  | signed : number_interpretation
+  | unsigned : number_interpretation
 
-instance : ToString value_t where
-  toString := value_t.convert_to_string
+inductive explicit_weak_id where
+  | invalid : explicit_weak_id
+  | potentially_valid : Int → explicit_weak_id
 
-def value_t.fromString (x: String) : Option value_t :=
-  match x with
-  | "uint8_t"     => uint8_t
-  | "uint16_t"    => uint16_t
-  | "uint32_t"    => uint32_t
-  | "int8_t"      => int8_t
-  | "int16_t"     => int16_t
-  | "int32_t"     => int32_t
-  | "float"       => float
-  | _             => Option.none
+inductive abstract_type where
+  | string : abstract_type
+  | bool : abstract_type
+  | void : abstract_type
+  | number : number_interpretation → word_size → abstract_type
+  | index : abstract_type
+  | indexed : abstract_type → abstract_type
+  | mapping : abstract_type → abstract_type → abstract_type
+  | function : abstract_type → (List abstract_type) → abstract_type
+  | strong_id : String → abstract_type
+  | god_object : abstract_type
 
+inductive named_variable where
+  | global_var : List String → named_variable
+  | local_var : String → named_variable
 
-inductive lua_type where
-  | id : String -> lua_type
-  | number : lua_type
-  | data_arrays : lua_type
+def typed_variable := named_variable×abstract_type
 
-def lua_type.convert_to_string (x : lua_type) : String :=
-  match x with
-  | id name => name ++ "_strong_id"
-  | number => "number"
-  | data_arrays => "data_arrays"
+inductive expression where
+  | term : typed_variable → expression
+  | call : expression → List expression → expression
+  | index : named_variable → expression -> expression
+  | projection : expression → String → expression
+  | explicit_numerical_value : Int → expression
 
-instance : ToString lua_type where
-  toString := lua_type.convert_to_string
+inductive instruction where
+  | assert : expression → instruction
+  | assignment : expression → expression → instruction
+  | return_value : expression → instruction
+  | function_declaration : named_variable → (List typed_variable) → List instruction → instruction
 
-def lua_type.fromString (x: String) : lua_type :=
-  match x with
-  | "uint8_t"     => number
-  | "uint16_t"    => number
-  | "uint32_t"    => number
-  | "int8_t"      => number
-  | "int16_t"     => number
-  | "int32_t"     => number
-  | "float"       => number
-  | s             => id s
+def program := List instruction
 
 structure raw_triple where
   column_type : String
   column_name : String
   column_target : String
 
-structure normal_type where
-  ffi_type : Option value_t
-  lua_type : Option lua_type
-
-structure field where
-  name : String
-  column_normal_type : normal_type
-
-structure link where
-  name : String
-  linked_table : String
 
 inductive column_type where
   | link_one : column_type
@@ -98,11 +73,40 @@ def column_type_to_str (a: column_type) : String :=
 instance : ToString column_type where
   toString := column_type_to_str
 
-structure table where
-  name : String
-  fields : List field
-  links_one : List link
-  links_many : List link
+
+def make_delete_row_program (table : table) : program :=
+  let table_namespace := namespace_name table.name
+
+  let function_var := named_variable.global_var [table_namespace, "delete"]
+
+  let table_key_t := abstract_type.strong_id table.name
+  let table_key_var := named_variable.local_var "id"
+  let table_key : typed_variable := ⟨ table_key_var, table_key_t ⟩
+
+  let state_t := abstract_type.god_object
+  let state_var := named_variable.global_var ["state"]
+  let state : typed_variable := ⟨ state_var, state_t ⟩
+
+  let is_fresh_fn_t := abstract_type.function abstract_type.bool [table_key_t]
+  let is_fresh_fn_var := named_variable.global_var [table_namespace, "is_fresh"]
+  let is_fresh_fn : typed_variable := ⟨is_fresh_fn_var, is_fresh_fn_t⟩
+
+  let is_used :=
+    expression.index
+      table_key_var
+      (expression.projection (expression.term state) s!"used_{table.name}_id")
+
+  let fresh_check := expression.call (expression.term is_fresh_fn) []
+  let declaration : instruction := instruction.function_declaration
+    function_var
+    [state, table_key]
+    [
+      instruction.assert fresh_check,
+      instruction.assignment is_used (expression.explicit_numerical_value 0)
+    ]
+  [
+    declaration
+  ]
 
 def validate_triples (x : List String) : IO Prop := do
   if x.length = 0 then
@@ -145,8 +149,8 @@ def table_append_tokens (target : table) (source : List String) : table :=
       | .link_many => table_append_tokens ⟨
           target.name,
           target.fields,
-          target.links_one.concat ⟨ name, c ⟩,
-          target.links_many
+          target.links_one,
+          target.links_many.concat ⟨ name, c ⟩
         ⟩ source
     | _, _ => target
   | _ => target
@@ -168,7 +172,6 @@ def string_to_table (name_raw : IO String) (x : IO String) : IO table := do
     fun (token : String) ↦ String.length token > 0
   pure (tokens_to_table name tokens)
 
-def namespace_name (x : String) : String := x.toUpper
 
 inductive lua_term where
   | var : String -> lua_term
@@ -180,11 +183,13 @@ def lua_term.toString (x : lua_term) :=
 inductive lua_callable_term where
   | getter: String -> String -> lua_callable_term
   | setter: String -> String -> lua_callable_term
+  -- | new_row: String -> lua_callable_term
 
 def lua_callable_term.toString (x : lua_callable_term) : String :=
   match x with
   | getter table field_name => namespace_name table ++ ".get_" ++ field_name
   | setter table field_name => namespace_name table ++ ".set_" ++ field_name
+  -- | new_row table => namespace_name table ++ ".create_" ++ table
 
 structure lua_variable where
   term : lua_term
@@ -227,6 +232,8 @@ def function_body (x : lua_function) : String :=
   | lua_callable_term.setter table field =>
     s!"\tassert(state.generation_counter_array_{table}[id.internal_id] == id.generation_counter)\n" ++
     s!"\tstate.data_array_{table}_{field}[id.internal_id] = value\n"
+  -- | lua_callable_term.new_row table =>
+
 
 def lua_function.convert_to_string (x : lua_function) : String :=
   ""
@@ -285,9 +292,24 @@ def link_one_to_lua (table_name : String) (data : List link) : String :=
     s!"---@param state {lua_type.data_arrays}\n" ++
     s!"local function reserve_link_array_{table_name}_{l.linked_table}(state)\n" ++
     s!"{tb}state.data_array_{table_name}_to_{l.linked_table} = ffi.new(\"int32_t[?]\", state.size_{table_name})\n" ++
-    s!"{tb}state.data_array_{table_name}_from_{l.linked_table} = ffi.new(\"int32_t[?]\", state.size_{l.linked_table})\n" ++
+    s!"{tb}state.data_array_{table_name}_one_from_{l.linked_table} = ffi.new(\"int32_t[?]\", state.size_{l.linked_table})\n" ++
     s!"end\n"
     ++ link_one_to_lua table_name data
+
+
+def link_many_to_lua (table_name : String) (data : List link) : String :=
+  match data with
+  | [] => ""
+  | l :: data =>
+    s!"---@param state {lua_type.data_arrays}\n" ++
+    s!"local function reserve_link_array_{table_name}_{l.linked_table}(state)\n" ++
+    s!"{tb}state.data_array_{table_name}_to_{l.linked_table} = ffi.new(\"int32_t[?]\", state.size_{table_name})\n" ++
+    s!"{tb}state.data_array_{table_name}_many_from_{l.linked_table} = {empty_table}\n" ++
+    s!"{tb}for i = 0, state.size_{l.linked_table} - 1 do\n" ++
+    s!"{tb}{tb}state.data_array_{table_name}_many_from_{l.linked_table}[i] = {empty_table}\n" ++
+    s!"{tb}end\n" ++
+    s!"end\n"
+    ++ link_many_to_lua table_name data
 
 def reserve_link_one (table_name : String) (data : List link) : String :=
   match data with
@@ -296,6 +318,13 @@ def reserve_link_one (table_name : String) (data : List link) : String :=
     s!"{tb}reserve_link_array_{table_name}_{l.linked_table}(state)\n"
     ++ reserve_link_one table_name data
 
+def reserve_link_many (table_name : String) (data : List link) : String :=
+  match data with
+  | [] => ""
+  | l :: data =>
+    s!"{tb}reserve_link_array_{table_name}_{l.linked_table}(state)\n"
+    ++ reserve_link_many table_name data
+
 def reserve_field (table_name : String) (data : List field) : String :=
   match data with
   | [] => ""
@@ -303,13 +332,71 @@ def reserve_field (table_name : String) (data : List field) : String :=
     s!"{tb}reserve_data_array_{table_name}_{f.name}(state)\n"
     ++ reserve_field table_name data
 
+def create_links_annotation (links : List link) : String :=
+  match links with
+  | [] => ""
+  | l :: links =>
+    s!"---@param {l.linked_table}_link {lua_type.id l.linked_table}\n"
+    ++ create_links_annotation links
+
+def create_links_args (links : List link) : String :=
+  match links with
+  | [] => ""
+  | l :: links =>
+    s!", {l.linked_table}_link"
+    ++ create_links_args links
+
+def create_links_one_action (table_name : String) (links : List link) : String :=
+  match links with
+  | [] => ""
+  | l :: links =>
+    s!"{tb}assert({namespace_name l.linked_table}.is_valid(state, {l.linked_table}_link))\n"
+    ++ s!"{tb}assert(state.data_array_{table_name}_one_from_{l.name}[{l.linked_table}_link.internal_id] == 0)\n"
+    ++ s!"{tb}state.data_array_{table_name}_to_{l.name}[id] = {l.linked_table}_link.internal_id\n"
+    ++ s!"{tb}state.data_array_{table_name}_one_from_{l.name}[{l.linked_table}_link.internal_id] = id\n"
+    ++ create_links_one_action table_name links
+
+
+def delete_links_one_action (table_name : String) (links : List link) : String :=
+  match links with
+  | [] => ""
+  | l :: links =>
+    s!"{tb}assert({namespace_name l.linked_table}.is_valid(state, {l.linked_table}_link))\n"
+    ++ s!"{tb}assert(state.data_array_{table_name}_one_from_{l.name}[{l.linked_table}_link.internal_id] == 0)\n"
+    ++ s!"{tb}state.data_array_{table_name}_to_{l.name}[id] = {l.linked_table}_link.internal_id\n"
+    ++ s!"{tb}state.data_array_{table_name}_one_from_{l.name}[{l.linked_table}_link.internal_id] = id\n"
+    ++ create_links_one_action table_name links
+
+def create_links_many_action (table_name : String) (links : List link) : String :=
+  match links with
+  | [] => ""
+  | l :: links =>
+    s!"{tb}assert({namespace_name l.linked_table}.is_valid(state, {l.linked_table}_link))\n"
+    ++ s!"{tb}state.data_array_{table_name}_to_{l.name}[id] = {l.linked_table}_link.internal_id\n"
+    ++ s!"{tb}state.data_array_{table_name}_many_from_{l.name}[{l.linked_table}_link.internal_id][id] = id\n"
+    ++ create_links_one_action table_name links
+
 def table_to_lua (data : IO table) : IO String := do
   let table ← data
+
   pure (
     "local ffi = require(\"ffi\")\n" ++
     s!"{namespace_name table.name} = " ++ "{}\n"
+
+    ++ s!"---@param state data_arrays\n"
+    ++ s!"---@param id {lua_type.id table.name}\n"
+    ++ s!"function {namespace_name table.name}.is_valid(state, id)\n"
+    ++ s!"{tb}local bounded = state.size_{table.name} > id.internal_id\n"
+    ++ s!"{tb}if (not bounded) then return false end\n"
+    ++ s!"{tb}local is_used = state.used_{table.name}_id[id.internal_id] == 1\n"
+    ++ s!"{tb}local fresh = state.generation_counter_array_{table.name}[id.internal_id] == id.generation_counter\n"
+    ++ s!"{tb}return bounded and is_used and fresh\n"
+    ++ s!"end\n"
+
     ++ s!"---@param state data_arrays\n"
     ++ s!"local function reserve_generation_array(state)\n"
+    ++ s!"{tb}state.available_{table.name}_id = 0\n"
+    ++ s!"{tb}state.used_{table.name}_id = ffi.new(\"uint8_t[?]\", state.size_{table.name})\n"
     ++ s!"{tb}state.generation_counter_array_{table.name} = ffi.new(\"int32_t[?]\", state.size_{table.name})\n"
     ++ s!"end\n"
     ++ s!"---@class {(lua_type.id table.name)}\n"
@@ -317,11 +404,39 @@ def table_to_lua (data : IO table) : IO String := do
     ++ s!"---@field generation_counter number\n\n"
     ++ fields_to_lua table.name table.fields
     ++ link_one_to_lua table.name table.links_one
+    ++ link_many_to_lua table.name table.links_many
     ++ s!"---@param state data_arrays\n"
     ++ s!"function {namespace_name table.name}.reserve(state)\n"
     ++ s!"{tb}reserve_generation_array(state)\n"
     ++ reserve_field table.name table.fields
     ++ reserve_link_one table.name table.links_one
+    ++ reserve_link_many table.name table.links_many
+    ++ "end\n"
+
+
+    ++ s!"---@param state data_arrays\n"
+    ++ create_links_annotation table.links_one
+    ++ create_links_annotation table.links_many
+    ++ s!"---@returns {lua_type.id table.name}\n"
+    ++ s!"function {namespace_name table.name}.create(state{create_links_args table.links_one}{create_links_args table.links_many})\n"
+    ++ s!"{tb}local id = state.available_{table.name}_id\n"
+    ++ s!"{tb}state.used_{table.name}_id[id] = 1\n"
+    ++ create_links_one_action table.name table.links_one
+    ++ create_links_many_action table.name table.links_many
+    ++ s!"{tb}while state.used_{table.name}_id[state.available_{table.name}_id] ~= 0 do\n"
+    ++ s!"{tb}{tb}assert(state.available_{table.name}_id < state.size_{table.name})\n"
+    ++ s!"{tb}{tb}state.available_{table.name}_id = state.available_{table.name}_id + 1\n"
+    ++ s!"{tb}end\n"
+    ++ s!"{tb}---@type {lua_type.id table.name}\n"
+    ++ s!"{tb}return ffi.new(\"struct strong_id\", {curly s!"id, state.generation_counter_array_{table.name}[id] "})\n"
+    ++ "end\n"
+
+    ++ s!"---@param state data_arrays\n"
+    ++ s!"---@param id {lua_type.id table.name}\n"
+    ++ s!"function {namespace_name table.name}.delete(state, id)\n"
+    ++ s!"{tb}assert({namespace_name table.name}.is_valid(state, id))\n"
+    ++ s!"{tb}state.used_{table.name}_id[id.internal_id] = 0\n"
+    ++ s!"{tb}if (id.internal_id < state.available_{table.name}_id) then state.available_{table.name}_id = id.internal_id end\n"
     ++ "end\n"
   )
 
@@ -349,10 +464,17 @@ def append_state_property_link_one (table_name : String) (links : List link) : S
   match links with
   | l :: links =>
     s!"---@field data_array_{table_name}_to_{l.name} number[]\n"++
-    s!"---@field data_array_{table_name}_from_{l.name} number[]\n"++
+    s!"---@field data_array_{table_name}_one_from_{l.name} number[]\n"++
     append_state_property_link_one table_name links
   | _ => ""
 
+def append_state_property_link_many (table_name : String) (links : List link) : String :=
+  match links with
+  | l :: links =>
+    s!"---@field data_array_{table_name}_to_{l.name} number[]\n"++
+    s!"---@field data_array_{table_name}_many_from_{l.name} (table<number, number>)[]\n"++
+    append_state_property_link_one table_name links
+  | _ => ""
 
 def state_fields (args: List String) : IO String := do
   match args with
@@ -361,10 +483,13 @@ def state_fields (args: List String) : IO String := do
     let text := IO.FS.readFile input_filename
     let table ← string_to_table table_name text
     let result : String :=
-      s!"---@field generation_counter_array_{table.name} number[]\n"++
-      s!"---@field size_{table.name} number\n"++
-      append_state_property_fields table.name table.fields ++
-      append_state_property_link_one table.name table.links_one
+      s!"---@field generation_counter_array_{table.name} number[]\n"
+      ++ s!"---@field size_{table.name} number\n"
+      ++ s!"---@field used_{table.name}_id number[]\n"
+      ++ s!"---@field available_{table.name}_id number\n"
+      ++ append_state_property_fields table.name table.fields
+      ++ append_state_property_link_one table.name table.links_one
+      ++ append_state_property_link_many table.name table.links_many
     let next_result ← state_fields args
     pure (result ++ next_result)
   | _ =>
@@ -383,5 +508,5 @@ def main (args : List String) : IO UInt32 := do
     IO.FS.writeFile ⟨ output_file⟩ (state_description ++ fields)
     pure 0
   | _ =>
-    IO.println s!"Error: Invalid arguments sequence"
+    IO.println s!"Error: Invalid arguments sequence\n"
     pure 1
