LeanLuaDataArrays/Language.lean
@@ -1,0 +1,243 @@
+namespace Pure
+
+inductive word_size where
+  | w1 : word_size
+  | w2 : word_size
+  | w4 : word_size
+
+inductive number_interpretation where
+  | signed : number_interpretation
+  | unsigned : number_interpretation
+
+inductive data_type where
+  | string : data_type
+  | bool : data_type
+  | number : number_interpretation → word_size → data_type
+  | void : data_type
+
+def int32_t := data_type.number number_interpretation.signed word_size.w4
+
+end Pure
+
+
+namespace Table
+
+structure field where
+  name : String
+  column_normal_type : Pure.data_type
+
+structure link where
+  name : String
+  linked_table : String
+
+structure reference where
+  referenced_as : String
+  referenced_in : String
+
+structure table where
+  name : String
+  fields : List field
+  links_one : List link
+  links_many : List link
+  references : List reference
+
+end Table
+
+namespace Language
+
+def god_object_name := "state"
+def validity_check_name := "is_valid"
+def id_s := "id"
+
+inductive Notion where
+  | validity_checker : String → Notion
+
+def namespace_name (x : String) : String := x.toUpper
+
+inductive SupposedType where
+  | pure : Pure.data_type → SupposedType
+  | alias : String → SupposedType
+  | index : SupposedType
+  | strong_id : String → SupposedType
+
+inductive GivenName where
+  | name : List String → String → GivenName
+
+inductive Thing where
+  | term : GivenName → Thing
+  | call : Thing → Thing → Thing
+  | index : Thing → Thing -> Thing
+  | projection : Thing → String → Thing
+  | explicit_numerical_value : Int → Thing
+  | explicit_boolean_value : Bool → Thing
+  | less_or_equal : Thing → Thing → Thing
+  | less : Thing → Thing → Thing
+  | equal : Thing → Thing → Thing
+  | and : Thing → Thing → Thing
+  | or : Thing → Thing → Thing
+  | list : List Thing → Thing
+
+structure StrongId (table_name : String) where
+  var : GivenName := GivenName.name [] s!"{table_name}_id"
+  expr := Thing.term var
+  internal_id : Thing := Thing.projection expr "internal_id"
+  generation : Thing := Thing.projection expr "generation"
+  type := SupposedType.strong_id table_name
+
+def ValueName : GivenName := GivenName.name [] "value"
+def ValueExpr : Thing := Thing.term ValueName
+
+inductive Instruction where
+  | assert : Thing → Instruction
+  | assignment : Thing → Thing → Instruction
+  | return_value : Thing → Instruction
+  | program : List Instruction → Instruction
+  | function_declaration :
+    GivenName
+    → SupposedType → (List (GivenName × SupposedType))
+    → Instruction
+    → Instruction
+  | condition : Thing → Instruction → Instruction → Instruction
+  | reserve_pure_array : Thing → Pure.data_type → Thing → Instruction
+
+def validity_checker (table_name : String) : Thing :=
+  Thing.term
+  (
+    GivenName.name
+    [namespace_name table_name]
+    validity_check_name
+  )
+
+structure DataArrays where
+  self
+    := GivenName.name [] "state"
+
+  self_t
+    := SupposedType.alias "data_arrays"
+
+  expr
+    := Thing.term (GivenName.name [] god_object_name)
+
+  size (table : String) : Thing
+    := Thing.projection expr s!"{table}_size"
+
+  usage_array (table: String) : Thing
+    := Thing.projection expr s!"{table}_usage"
+
+  generation_array (table: String) : Thing
+    := Thing.projection expr s!"{table}_generation"
+
+  field_array (table: String) (field : String) : Thing
+    := Thing.projection expr s!"{table}_data_{field}"
+
+  usage (table: String) (id : StrongId table) : Thing
+    := Thing.index (usage_array table) (id.internal_id)
+
+  generation (table: String) (id : StrongId table) : Thing
+    := Thing.index (generation_array table) (id.internal_id)
+
+  field (table: String) (field : String) (id : StrongId table) : Thing
+    := Thing.index (field_array table field) (id.internal_id)
+
+
+
+def Validity (table_name : String) (id : StrongId table_name) : Thing :=
+  Thing.call (validity_checker table_name) (Thing.list [id.expr])
+
+def IsValid (data : DataArrays) (table_name : String) (id : StrongId table_name) : Instruction :=
+  let in_bounds := Thing.less id.internal_id (data.size table_name)
+  let is_fresh := Thing.equal id.generation (data.generation table_name id)
+  Instruction.program [
+    Instruction.condition
+      in_bounds
+      (Instruction.return_value (Thing.and in_bounds is_fresh))
+      (Instruction.return_value (Thing.explicit_boolean_value False))
+  ]
+
+def IsValidFunc (data : DataArrays) (table_name : String) (id : StrongId table_name) : Instruction :=
+  Instruction.function_declaration
+    (GivenName.name [namespace_name table_name] validity_check_name)
+    (SupposedType.pure Pure.data_type.bool)
+    [
+      ⟨ data.self, data.self_t ⟩,
+      ⟨ id.var, id.type ⟩
+    ]
+    (IsValid data table_name id)
+
+def AccessFieldFunc (data : DataArrays) (table_name : String) (id : StrongId table_name) (field : Table.field) : Instruction :=
+  Instruction.function_declaration
+    (GivenName.name [namespace_name table_name] ("get_" ++ field.name))
+    (SupposedType.pure field.column_normal_type)
+    [
+      ⟨ data.self, data.self_t ⟩,
+      ⟨ id.var, id.type ⟩
+    ]
+    (
+      Instruction.program
+      [
+        Instruction.assert (Validity table_name id),
+        Instruction.return_value (data.field table_name field.name id)
+      ]
+    )
+
+def ChangeFieldFunc (data : DataArrays) (table_name : String) (id : StrongId table_name) (field : Table.field) : Instruction :=
+  Instruction.function_declaration
+    (GivenName.name [namespace_name table_name] ("set_" ++ field.name))
+    (SupposedType.pure Pure.data_type.void)
+    [
+      ⟨ data.self, data.self_t ⟩,
+      ⟨ id.var, id.type ⟩,
+      ⟨ ValueName, SupposedType.pure field.column_normal_type ⟩
+    ]
+    (
+      Instruction.program
+      [
+        Instruction.assert (Validity table_name id),
+        Instruction.assignment (data.field table_name field.name id) ValueExpr
+      ]
+    )
+
+def SetSizeFunc (data : DataArrays) (table_name : String) : Instruction :=
+  Instruction.function_declaration
+    (GivenName.name [namespace_name table_name] ("resize"))
+    (SupposedType.pure Pure.data_type.void)
+    [
+      ⟨ data.self, data.self_t ⟩,
+      ⟨ ValueName, SupposedType.pure (Pure.data_type.number Pure.number_interpretation.signed Pure.word_size.w4) ⟩
+    ]
+    (
+      Instruction.program
+      [
+        Instruction.assignment (data.size table_name) ValueExpr
+      ]
+    )
+
+def ReserveArraysFunc (data : DataArrays) (table : Table.table) : Instruction :=
+  Instruction.function_declaration
+    (GivenName.name [namespace_name table.name] ("reserve"))
+    (SupposedType.pure Pure.data_type.void)
+    [
+      ⟨ data.self, data.self_t ⟩
+    ]
+    (
+      Instruction.program
+      [
+        Instruction.reserve_pure_array (data.usage_array table.name) Pure.int32_t (data.size table.name)
+      ]
+    )
+
+def Language := (indent : String) → (i : Instruction) → String
+
+def Translate (t: Table.table) (l: Language) : String :=
+  let state : DataArrays := {}
+  let id : StrongId t.name := {}
+
+  let l' := l ""
+
+  l' (Instruction.program [IsValidFunc state t.name id])
+  ++
+  l' (Instruction.program (t.fields.map (AccessFieldFunc state t.name id)))
+  ++
+  l' (Instruction.program (t.fields.map (ChangeFieldFunc state t.name id)))
+
+end Language
