LeanLuaDataArrays/Lua.lean
@@ -1,0 +1,199 @@
+import LeanLuaDataArrays.Language
+
+namespace AnnotatedLuajit
+
+open Language
+
+
+inductive ffi_type where
+  | uint8_t : ffi_type
+  | uint16_t : ffi_type
+  | uint32_t : ffi_type
+  | int8_t : ffi_type
+  | int16_t : ffi_type
+  | int32_t : ffi_type
+  | float : ffi_type
+  | bool : ffi_type
+
+def ffi_type.convert_to_string (x: ffi_type) : String :=
+  match x with
+  | uint8_t     => "uint8_t"
+  | uint16_t    => "uint16_t"
+  | uint32_t    => "uint32_t"
+  | int8_t      => "int8_t"
+  | int16_t     => "int16_t"
+  | int32_t     => "int32_t"
+  | float       => "float"
+  | bool        => "bool"
+
+
+instance : ToString ffi_type where
+  toString := ffi_type.convert_to_string
+
+def ffi_type.fromString (x: String) : Option ffi_type :=
+  match x with
+  | "uint8_t"     => uint8_t
+  | "uint16_t"    => uint16_t
+  | "uint32_t"    => uint32_t
+  | "int8_t"      => int8_t
+  | "int16_t"     => int16_t
+  | "int32_t"     => int32_t
+  | "float"       => float
+  | "bool"        => bool
+  | _             => Option.none
+
+theorem FFI_string_conversion_is_valid (x : ffi_type) : (ffi_type.fromString x.convert_to_string) = x := by
+  cases x
+  repeat rfl
+
+
+inductive lua_type where
+  | id : String -> lua_type
+  | number : lua_type
+  | data_arrays : lua_type
+
+def lua_type.convert_to_string (x : lua_type) : String :=
+  match x with
+  | id name => name ++ "_strong_id"
+  | number => "number"
+  | data_arrays => "data_arrays"
+
+instance : ToString lua_type where
+  toString := lua_type.convert_to_string
+
+def lua_type.fromString (x: String) : lua_type :=
+  match x with
+  | "uint8_t"     => number
+  | "uint16_t"    => number
+  | "uint32_t"    => number
+  | "int8_t"      => number
+  | "int16_t"     => number
+  | "int32_t"     => number
+  | "float"       => number
+  | s             => id s
+
+def ConvertTypeLua (t : SupposedType) : String :=
+  match t with
+  | SupposedType.index => "number"
+  | SupposedType.alias name => name
+  | SupposedType.strong_id table => table ++ "_strong_id"
+  | SupposedType.pure pure_type =>
+    match pure_type with
+    | Pure.data_type.bool => "boolean"
+    | Pure.data_type.number .. => "number"
+    | Pure.data_type.string => "string"
+    | Pure.data_type.void => "error_type"
+
+def ConvertTypeFFI (pure_type : Pure.data_type) : Option ffi_type :=
+  match pure_type with
+  | Pure.data_type.bool => ffi_type.bool
+  | Pure.data_type.number interpretation size =>
+    match interpretation with
+    | Pure.number_interpretation.signed =>
+      match size with
+      | Pure.word_size.w1 => ffi_type.int8_t
+      | Pure.word_size.w2 => ffi_type.int16_t
+      | Pure.word_size.w4 => ffi_type.int32_t
+    | Pure.number_interpretation.unsigned =>
+      match size with
+      | Pure.word_size.w1 => ffi_type.uint8_t
+      | Pure.word_size.w2 => ffi_type.uint16_t
+      | Pure.word_size.w4 => ffi_type.uint32_t
+  | Pure.data_type.string => none
+  | Pure.data_type.void => none
+
+def ResolveNamespace (n : List String) : String :=
+  match n with
+  | item :: n => item ++ "." ++ ResolveNamespace n
+  | [] => ""
+
+def ResolveName (n : GivenName) : String :=
+  match n with
+  | GivenName.name namespace_chain name => ResolveNamespace namespace_chain ++ name
+
+def Signify (t : Thing) : String :=
+  match t with
+  | Thing.and a b => s!"({Signify a} and {Signify b})"
+  | Thing.or a b => s!"({Signify a} and {Signify b})"
+  | Thing.call f l => s!"{Signify f}({Signify l})"
+  | Thing.equal a b => s!"({Signify a} == {Signify b})"
+  | Thing.explicit_boolean_value p =>
+    match p with
+    | Bool.true => "true"
+    | Bool.false => "false"
+  | Thing.explicit_numerical_value a => s!"{a}"
+  | Thing.index a b => s!"{Signify a}[{Signify b}]"
+  | Thing.less a b => s!"({Signify a} < {Signify b})"
+  | Thing.less_or_equal a b => s!"({Signify a} <= {Signify b})"
+  | Thing.list l =>
+    match l with
+    | [] => ""
+    | [a] => s!"{Signify a}"
+    | a :: l => s!"{Signify a}, {Signify (Thing.list l)}"
+  | Thing.projection a s => s!"{Signify a}.{s}"
+  | Thing.term a => ResolveName a
+
+def ResolveParamTypes (params: List (GivenName × SupposedType)) :=
+  match params with
+  | [] => ""
+  | ⟨var, var_t⟩ :: params =>
+    (
+      match var with
+      | GivenName.name _ name => s!"---@param {name} {ConvertTypeLua var_t}\n"
+    )
+    ++ ResolveParamTypes params
+
+def ResolveParams (params: List (GivenName × SupposedType)) :=
+  match params with
+  | [] => ""
+  | [⟨var, _⟩] =>
+    match var with
+    | GivenName.name _ name => name
+  | ⟨var, _⟩ :: params =>
+    match var with
+    | GivenName.name _ name => name ++ ", " ++ ResolveParams params
+
+def JoinLines (lines : List String) :=
+  match lines with
+  | [] => ""
+  | line :: lines => s!"{line}\n" ++ JoinLines lines
+
+def Compile (tb : String) (indent : String) (i : Instruction) : String :=
+  match i with
+  | Instruction.return_value e => s!"{indent}return {Signify e}\n"
+
+  | Instruction.assert e => s!"{indent}assert({Signify e})\n"
+
+  | Instruction.condition a b c =>
+    s!"{indent}if {Signify a} then\n"
+    ++(Compile tb s!"{indent}{tb}" b)
+    ++"{indent}else\n"
+    ++(Compile tb s!"{indent}{tb}" c)
+
+  | Instruction.assignment a b => s!"{Signify a} = {Signify b}"
+
+  | Instruction.function_declaration name out_type params body =>
+    match out_type with
+    | SupposedType.pure Pure.data_type.void =>
+      ResolveParamTypes params
+      ++ s!"{indent}function {ResolveName name}({ResolveParams params})"
+      ++ Compile tb s!"{indent}{tb}" body
+      ++ s!"end"
+    | _ =>
+      ResolveParamTypes params
+      ++ s! "---@returns {ConvertTypeLua out_type}"
+      ++ s!"{indent}function {ResolveName name}({ResolveParams params})"
+      ++ Compile tb s!"{indent}{tb}" body
+      ++ s!"end"
+
+  | Instruction.program p => JoinLines (p.map (Compile tb indent))
+
+  | Instruction.reserve_pure_array array data_type size =>
+    let ffi_type := ConvertTypeFFI data_type
+    match ffi_type with
+    | none => ""
+    | some x =>
+      s!"{Signify array} = ffi.new(\"{x}[?]\", {Signify size})"
+
+
+end AnnotatedLuajit
